WIP: trying to define cc_compose between different callconv in VerComp.v

unusedglob/VerComp.v
@@ -11,6 +11,239 @@ Require Import Inject InjectFootprint.
 Require Import CKLRAlgebra.
 Require Import Callconv ForwardSim.
 
+
+(** * Test1: cc_compose_1 *)
+
+
+Program Definition cc_compose_1 {li1 li2 li3} (cc12: callconv li1 li2) (cc23: callconv' li2 li3) :=
+  {|
+    ccworld' := Genv.symtbl * ccworld cc12 * ccworld' cc23;
+    match_senv' '(se2, w12, w23) se1 se3 :=
+      match_senv cc12 w12 se1 se2 /\
+      match_senv' cc23 w23 se2 se3;
+    match_query' '(se2, w12, w23) q1 q3 :=
+      exists q2,
+        match_query cc12 w12 q1 q2 /\
+        match_query' cc23 w23 q2 q3;
+    match_reply' '(se2, w12, w23) r1 r3 :=
+      exists r2,
+        match_reply cc12 w12 r1 r2 /\
+        match_reply' cc23 w23 r2 r3;
+  |}.
+Next Obligation.
+  etransitivity.
+  eapply match_senv_public_preserved'. eauto.
+  eauto using match_senv_public_preserved.
+Qed.
+
+Infix "@1" := cc_compose_1 (at level 30, right associativity) : cc_scope.
+
+
+Section CC_COMPOSE1.
+
+Context {liA1 liA2 liA3} {ccA12: callconv liA1 liA2} {ccA23: callconv' liA2 liA3}.
+Context {liB1 liB2 liB3} {ccB12: callconv liB1 liB2} {ccB23: callconv' liB2 liB3}.
+Context (L1: semantics liA1 liB1) (L2: semantics liA2 liB2) (L3: semantics liA3 liB3).
+
+
+Lemma compose_fsim_components_1:
+  fsim_components ccA12 ccB12 L1 L2 ->
+  fsim_components' ccA23 ccB23 L2 L3 ->
+  fsim_components' (cc_compose_1 ccA12 ccA23) (cc_compose_1 ccB12 ccB23) L1 L3.
+Proof.
+  intros [index order match_states Hsk props order_wf].
+  intros [index' order' match_states' Hsk' props' order_wf'].
+  set (ff_index := (index' * index)%type).
+  set (ff_order := lex_ord (clos_trans _ order') order).
+  set (ff_match_states :=
+         fun se1 se3 '(se2, w, w') (i: ff_index) (s1: state L1) (s3: state L3) =>
+           exists s2,
+             match_states se1 se2 w (snd i) s1 s2 /\
+             match_states' se2 se3 w' (fst i) s2 s3).
+  apply Forward_simulation' with ff_order ff_match_states.
+  3: { unfold ff_order. auto using wf_lex_ord, wf_clos_trans. }
+  1: { rewrite Hsk. congruence. }
+  intros se1 se3 [[se2 w] w'] (Hse12 & Hse23) Hse1. cbn in *.
+  destruct Hse1 as [Hvalid1 [Hvalid3 COMPAT13]].
+  assert (Hvalid2: Genv.valid_for (skel L2) se2).
+  { rewrite <- Hsk. eapply match_senv_valid_for; eauto. }
+  assert (Hse2: Genv.skel_symtbl_compatible (skel L2) (skel L3) se2 se3).
+  {
+    constructor; eauto. split. eauto.
+    destruct COMPAT13.
+    split. intros. rewrite <- Hsk in H1. eauto.
+    intro. apply H0. red.
+    destruct H1 as [b1 [A B]].
+    admit. (*need more requirement about main of general match_senv*)
+  }
+  constructor.
+- (* valid query *)
+  intros q1 q3 (q2 & Hq12 & Hq23).
+  erewrite fsim_match_valid_query'. 2: eapply props'; eauto.
+  eapply fsim_match_valid_query; eauto. eauto.
+- (* initial states *)
+  intros q1 q3 s1 (q2 & Hq12 & Hq23) Hs1.
+  edestruct (@fsim_match_initial_states liA1) as (i & s2 & A & B); eauto.
+  edestruct (@fsim_match_initial_states' liA2) as (i' & s3 & C & D); eauto.
+  exists (i', i); exists s3; split; auto. exists s2; auto.
+- (* final states *)
+  intros. cbn. destruct H as (s3 & A & B).
+  edestruct (@fsim_match_final_states liA1) as (r2 & Hr2 & Hr12); eauto.
+  edestruct (@fsim_match_final_states' liA2) as (r3 & Hr3 & Hr23); eauto.
+- (* external states *)
+  intros. destruct H as [s3 [A B]].
+  edestruct (@fsim_match_external liA1) as (w12 & q2 & Hq2 & Hq12 & Hw12 & Hk12); eauto.
+  edestruct (@fsim_match_external' liA2) as (w23 & q3 & Hq3 & Hq23 & Hw23 & Hk23); eauto.
+  exists (se2, w12, w23), q3. cbn; repeat apply conj; eauto.
+  intros r1 r3 s1' (r2 & Hr12 & Hr23) Hs1'.
+  edestruct Hk12 as (i12' & s2' & Hs2' & Hs12'); eauto.
+  edestruct Hk23 as (i23' & s3' & Hs3' & Hs23'); eauto.
+  exists (i23', i12'), s3'. split; auto. exists s2'; auto.
+- (* simulation *)
+  intros. destruct H0 as [s3 [A B]]. destruct i as [i2 i1]; simpl in *.
+  edestruct (@fsim_simulation' liA1) as [(i1' & s3' & C & D) | (i1' & C & D & E)]; eauto.
++ (* L2 makes one or several steps. *)
+  edestruct (@simulation_plus' liA2) as [(i2' & s2' & P & Q) | (i2' & P & Q & R)]; eauto.
+* (* L3 makes one or several steps *)
+  exists (i2', i1'); exists s2'; split. auto. exists s3'; auto.
+* (* L3 makes no step *)
+  exists (i2', i1'); exists s2; split.
+  right; split. subst t; apply star_refl. red. left. auto.
+  exists s3'; auto.
++ (* L2 makes no step *)
+  exists (i2, i1'); exists s2; split.
+  right; split. subst t; apply star_refl. red. right. auto.
+  exists s3; auto.
+Admitted.
+
+
+Lemma compose_forward_simulations_1:
+  forward_simulation ccA12 ccB12 L1 L2 ->
+  forward_simulation' ccA23 ccB23 L2 L3 ->
+  forward_simulation' (cc_compose_1 ccA12 ccA23) (cc_compose_1 ccB12 ccB23) L1 L3.
+Proof.
+  intros [X] [Y]. constructor.
+  apply compose_fsim_components_1; auto.
+Qed.
+
+End CC_COMPOSE1.
+
+
+Program Definition cc_compose_2 {li1 li2 li3} (cc12: callconv' li1 li2) (cc23: callconv li2 li3) :=
+  {|
+    ccworld' := Genv.symtbl * ccworld' cc12 * ccworld cc23;
+    match_senv' '(se2, w12, w23) se1 se3 :=
+      match_senv' cc12 w12 se1 se2 /\
+      match_senv cc23 w23 se2 se3;
+    match_query' '(se2, w12, w23) q1 q3 :=
+      exists q2,
+        match_query' cc12 w12 q1 q2 /\
+        match_query cc23 w23 q2 q3;
+    match_reply' '(se2, w12, w23) r1 r3 :=
+      exists r2,
+        match_reply' cc12 w12 r1 r2 /\
+        match_reply cc23 w23 r2 r3;
+  |}.
+Next Obligation.
+  etransitivity.
+  eapply match_senv_public_preserved; eauto.
+  eauto using match_senv_public_preserved'.
+Qed.
+
+Infix "@2" := cc_compose_1 (at level 30, right associativity) : cc_scope.
+
+
+Section CC_COMPOSE2.
+
+Context {liA1 liA2 liA3} {ccA12: callconv' liA1 liA2} {ccA23: callconv liA2 liA3}.
+Context {liB1 liB2 liB3} {ccB12: callconv' liB1 liB2} {ccB23: callconv liB2 liB3}.
+Context (L1: semantics liA1 liB1) (L2: semantics liA2 liB2) (L3: semantics liA3 liB3).
+
+
+Lemma compose_fsim_components_2:
+  fsim_components' ccA12 ccB12 L1 L2 ->
+  fsim_components ccA23 ccB23 L2 L3 ->
+  fsim_components' (cc_compose_2 ccA12 ccA23) (cc_compose_2 ccB12 ccB23) L1 L3.
+Proof.
+  intros [index order match_states Hsk props order_wf].
+  intros [index' order' match_states' Hsk' props' order_wf'].
+  set (ff_index := (index' * index)%type).
+  set (ff_order := lex_ord (clos_trans _ order') order).
+  set (ff_match_states :=
+         fun se1 se3 '(se2, w, w') (i: ff_index) (s1: state L1) (s3: state L3) =>
+           exists s2,
+             match_states se1 se2 w (snd i) s1 s2 /\
+             match_states' se2 se3 w' (fst i) s2 s3).
+  apply Forward_simulation' with ff_order ff_match_states.
+  3: { unfold ff_order. auto using wf_lex_ord, wf_clos_trans. }
+  1: { rewrite <- Hsk'. congruence. }
+  intros se1 se3 [[se2 w] w'] (Hse12 & Hse23) Hse1. cbn in *.
+  destruct Hse1 as [Hvalid1 [Hvalid3 COMPAT13]].
+  assert (Hvalid2: Genv.valid_for (skel L2) se2).
+  { rewrite <- Hsk. eapply match_senv_valid_for; eauto. }
+  assert (Hse2: Genv.skel_symtbl_compatible (skel L2) (skel L3) se2 se3).
+  {
+    constructor; eauto. split. eauto.
+    destruct COMPAT13.
+    split. intros. rewrite <- Hsk in H1. eauto.
+    intro. apply H0. red.
+    destruct H1 as [b1 [A B]].
+    admit. (*need more requirement about main of general match_senv*)
+  }
+  constructor.
+- (* valid query *)
+  intros q1 q3 (q2 & Hq12 & Hq23).
+  erewrite fsim_match_valid_query'. 2: eapply props'; eauto.
+  eapply fsim_match_valid_query; eauto. eauto.
+- (* initial states *)
+  intros q1 q3 s1 (q2 & Hq12 & Hq23) Hs1.
+  edestruct (@fsim_match_initial_states liA1) as (i & s2 & A & B); eauto.
+  edestruct (@fsim_match_initial_states' liA2) as (i' & s3 & C & D); eauto.
+  exists (i', i); exists s3; split; auto. exists s2; auto.
+- (* final states *)
+  intros. cbn. destruct H as (s3 & A & B).
+  edestruct (@fsim_match_final_states liA1) as (r2 & Hr2 & Hr12); eauto.
+  edestruct (@fsim_match_final_states' liA2) as (r3 & Hr3 & Hr23); eauto.
+- (* external states *)
+  intros. destruct H as [s3 [A B]].
+  edestruct (@fsim_match_external liA1) as (w12 & q2 & Hq2 & Hq12 & Hw12 & Hk12); eauto.
+  edestruct (@fsim_match_external' liA2) as (w23 & q3 & Hq3 & Hq23 & Hw23 & Hk23); eauto.
+  exists (se2, w12, w23), q3. cbn; repeat apply conj; eauto.
+  intros r1 r3 s1' (r2 & Hr12 & Hr23) Hs1'.
+  edestruct Hk12 as (i12' & s2' & Hs2' & Hs12'); eauto.
+  edestruct Hk23 as (i23' & s3' & Hs3' & Hs23'); eauto.
+  exists (i23', i12'), s3'. split; auto. exists s2'; auto.
+- (* simulation *)
+  intros. destruct H0 as [s3 [A B]]. destruct i as [i2 i1]; simpl in *.
+  edestruct (@fsim_simulation' liA1) as [(i1' & s3' & C & D) | (i1' & C & D & E)]; eauto.
++ (* L2 makes one or several steps. *)
+  edestruct (@simulation_plus' liA2) as [(i2' & s2' & P & Q) | (i2' & P & Q & R)]; eauto.
+* (* L3 makes one or several steps *)
+  exists (i2', i1'); exists s2'; split. auto. exists s3'; auto.
+* (* L3 makes no step *)
+  exists (i2', i1'); exists s2; split.
+  right; split. subst t; apply star_refl. red. left. auto.
+  exists s3'; auto.
++ (* L2 makes no step *)
+  exists (i2, i1'); exists s2; split.
+  right; split. subst t; apply star_refl. red. right. auto.
+  exists s3; auto.
+Admitted.
+
+
+Lemma compose_forward_simulations_1:
+  forward_simulation ccA12 ccB12 L1 L2 ->
+  forward_simulation' ccA23 ccB23 L2 L3 ->
+  forward_simulation' (cc_compose_1 ccA12 ccA23) (cc_compose_1 ccB12 ccB23) L1 L3.
+Proof.
+  intros [X] [Y]. constructor.
+  apply compose_fsim_components_1; auto.
+Qed.
+
+End CC_COMPOSE1.
+
+
+
 (** * Test1: compose injp' ⋅ injp' = injp' *)
 
 (*
@@ -18,6 +251,10 @@ L1 <=injp'->injp' L2 ->
 L2 <=injp'->injp' L3 ->
 L1 <= injp'-> injp' L3
 *)
+
+
+
+
 
 Section COMPOSE_FORWARD_SIMULATIONS.
 
